core/Certification.v
@@ -161,7 +161,7 @@ Lemma tr_applyUnitOnPiece_leaf :
 forall (tr: Transformation) (sm : SourceModel) (sp: InputPiece) (te: TargetElementType) 
        (i:nat) (opu: OutputPatternUnit),
   evalOutputPatternElement opu sm sp i = Some te ->
-  applyUnitOnPiece opu tr sm sp i = optionListToList (evalOutputPatternLink sm sp te i (convert2 (traceTrOnModel tr sm)) opu).
+  applyUnitOnPiece opu tr sm sp i = evalOutputPatternLink sm sp te i (convert2 (traceTrOnModel tr sm)) opu.
 Proof.
   intros.
   destruct (evalOutputPatternLink sm sp te i (convert2 (traceTrOnModel tr sm)) opu) eqn:dst.
