transformations/Class2Relational/Class2RelationalAbstract.v
@@ -57,12 +57,12 @@ Definition Class2Relational :=
         [buildOutputPatternUnit "tab"
           (makeElement [Class_K] Table_K
             (fun i m c => Build_Table_t (class_id c) (class_name c)))
-            (makeLink [Class_K] Table_K TableColumns_K
+            (Parser.dropToList(makeLink [Class_K] Table_K TableColumns_K
             (fun tls i m c t =>
               attrs <- getClassAttributes c m;
               cols <- resolveAll tls "col" Column_K 
                 (singletons (map (ClassMetamodel.lift_EKind Attribute_K) attrs));
-              return Build_TableColumns_t t cols))
+              return Build_TableColumns_t t cols)))
         ];
       buildRule "Attribute2Column"
         (makeGuard [Attribute_K] (fun m a => negb (derived a)))
@@ -70,10 +70,10 @@ Definition Class2Relational :=
         [buildOutputPatternUnit "col"
           (makeElement [Attribute_K] Column_K
             (fun i m a => Build_Column_t (attr_id a) (attr_name a)))
-            (makeLink [Attribute_K] Column_K ColumnReference_K
+            (Parser.dropToList(makeLink [Attribute_K] Column_K ColumnReference_K
               (fun tls i m a c =>
                 cl <- getAttributeType a m;
                 tb <- resolve tls "tab" Table_K [ClassMetamodel.lift_EKind Class_K cl];
-                return Build_ColumnReference_t c tb))
+                return Build_ColumnReference_t c tb)))
         ]
     ].
